lifting.v
@@ -1,0 +1,143 @@
+From iris.program_logic Require Export weakestpre.
+From iris.program_logic Require Import ownership ectx_lifting. (* for ownP *)
+From lrust Require Export lang.
+From lrust Require Import tactics.
+From iris.proofmode Require Import weakestpre.
+Import uPred.
+Local Hint Extern 0 (head_reducible _ _) => do_head_step eauto 2.
+
+Section lifting.
+Context {Σ : iFunctor}.
+Implicit Types P Q : iProp lrust_lang Σ.
+Implicit Types Φ : val → iProp lrust_lang Σ.
+Implicit Types ef : option (expr []).
+
+(** Bind. This bundles some arguments that wp_ectx_bind leaves as indices. *)
+Lemma wp_bind {E e} K Φ :
+  WP e @ E {{ v, WP fill K (of_val v) @ E {{ Φ }} }} ⊢ WP fill K e @ E {{ Φ }}.
+Proof. exact: wp_ectx_bind. Qed.
+
+Lemma wp_bindi {E e} Ki Φ :
+  WP e @ E {{ v, WP fill_item Ki (of_val v) @ E {{ Φ }} }} ⊢
+     WP fill_item Ki e @ E {{ Φ }}.
+Proof. exact: weakestpre.wp_bind. Qed.
+
+(** Base axioms for core primitives of the language: Stateful reductions. *)
+Lemma wp_alloc_pst E σ n Φ :
+  0 < n →
+  (▷ ownP σ ★
+   ▷ (∀ l σ', (∀ i, σ !! (l.1, i) = None) ∧ ■ init_mem_spec l n σ σ' ∧ ownP σ'
+            -★ Φ (LitV $ LitLoc l)))
+  ⊢ WP Alloc (Lit $ LitInt n) @ E {{ Φ }}.
+Proof.
+  iIntros {?}  "[HP HΦ]".
+  set (φ (e' : expr []) σ' ef := ∃ l,
+          ef = None ∧ e' = Lit (LitLoc l) ∧ init_mem_spec l n σ σ' ∧
+          (∀ i, σ !! (l.1, i) = None)).
+  iApply (wp_lift_atomic_head_step (Alloc $ Lit $ LitInt n) φ σ);
+    try (by simpl; eauto).
+  { intros; subst φ; inv_head_step; eauto 8 using init_mem_sound. }
+  iFrame "HP". iNext. iIntros {v2 σ2 ef} "[Hφ HP]".
+  iDestruct "Hφ" as %(l & -> & [= <-]%of_to_val_flip & ? & ?); simpl.
+  iSplit; last done. iApply "HΦ". repeat iSplit; auto.
+Qed.
+
+Lemma wp_free_pst E σ l n Φ :
+  0 < n →
+  (∀ i, is_Some (σ !! (l.1, i)) ↔ (l.2 ≤ i ∧ i < l.2 + n)) →
+  (▷ ownP σ ★
+   ▷ (∀ l σ', ■ free_mem_spec l n σ σ' ∧ ownP σ'
+              -★ Φ (LitV $ LitUnit)))
+  ⊢ WP Free (Lit $ LitInt n) (Lit $ LitLoc l) @ E {{ Φ }}.
+Proof.
+  iIntros {??}  "[HP HΦ]".
+  set (φ (e' : expr []) σ' ef :=
+          ef = None ∧ e' = Lit LitUnit ∧ free_mem_spec l n σ σ').
+  iApply (wp_lift_atomic_head_step (Free (Lit $ LitInt n) (Lit $ LitLoc l)) φ σ);
+    try (by simpl; eauto).
+  { intros; subst φ; inv_head_step; eauto 8 using free_mem_sound. }
+  iFrame "HP". iNext. iIntros {v2 σ2 ef} "[Hφ HP]".
+  iDestruct "Hφ" as %(-> & [= <-]%of_to_val_flip & ?); simpl.
+  iSplit; last done. iApply "HΦ". repeat iSplit; auto.
+Qed.
+
+Lemma wp_read_sc_pst E σ l v Φ :
+  σ !! l = Some (RSt 0, v) →
+  (▷ ownP σ ★ ▷ (ownP σ -★ Φ v)) ⊢ WP Read ScOrd $ Lit $ LitLoc l @ E {{ Φ }}.
+Proof.
+  intros. rewrite -(wp_lift_atomic_det_head_step σ v σ None) ?right_id //.
+  intros; inv_head_step; eauto using to_of_val.
+Qed.
+
+Lemma wp_store_sc_pst E σ l e v v' Φ :
+  to_val e = Some v →
+  σ !! l = Some (RSt 0, v') →
+  (▷ ownP σ ★ ▷ (ownP (<[l:=(RSt 0, v)]>σ) -★ Φ (LitV LitUnit)))
+  ⊢ WP Write ScOrd (Lit (LitLoc l)) e @ E {{ Φ }}.
+Proof.
+  intros.
+  rewrite-(wp_lift_atomic_det_head_step σ (LitV LitUnit)
+             (<[l:=(RSt 0, v)]>σ) None) ?right_id //=. eauto.
+  intros; inv_head_step; eauto.
+Qed.
+
+Lemma wp_cas_fail_pst E σ l z1 z2 z' Φ :
+  σ !! l = Some (RSt 0, LitV $ LitInt z') → z' ≠ z1 →
+  (▷ ownP σ ★ ▷ (ownP σ -★ Φ (LitV $ LitInt 0)))
+  ⊢ WP CAS (Lit $ LitLoc l) (Lit $ LitInt z1) (Lit $ LitInt z2) @ E {{ Φ }}.
+Proof.
+  intros.
+  rewrite-(wp_lift_atomic_det_head_step σ (LitV $ LitInt 0) σ None) ?right_id //.
+  intros; inv_head_step; eauto.
+Qed.
+
+Lemma wp_cas_suc_pst E σ l z1 z2 Φ :
+  σ !! l = Some (RSt 0, LitV $ LitInt z1) →
+  (▷ ownP σ ★ ▷ (ownP (<[l:=(RSt 0, LitV $ LitInt z2)]>σ) -★ Φ (LitV $ LitInt 1)))
+  ⊢ WP CAS (Lit $ LitLoc l) (Lit $ LitInt z1) (Lit $ LitInt z2) @ E {{ Φ }}.
+Proof.
+  intros.
+  rewrite -(wp_lift_atomic_det_head_step σ (LitV $ LitInt 1)
+              (<[l:=(RSt 0, LitV $ LitInt z2 )]>σ) None) ?right_id //.
+  intros; inv_head_step; eauto.
+Qed.
+
+(** Base axioms for core primitives of the language: Stateless reductions *)
+Lemma wp_fork E e Φ :
+  (▷ Φ (LitV LitUnit) ★ ▷ WP e {{ _, True }}) ⊢ WP Fork e @ E {{ Φ }}.
+Proof.
+  rewrite -(wp_lift_pure_det_head_step (Fork e) (Lit LitUnit) (Some e)) //=.
+  rewrite later_sep -(wp_value _ _ (Lit _)) //.
+  intros; inv_head_step; eauto.
+Qed.
+
+Lemma wp_rec E f xl erec erec' e el Φ :
+  e = Rec f xl erec →
+  List.Forall (λ ei, is_Some (to_val ei)) el →
+  subst_l xl el erec = Some erec' →
+  ▷ WP subst f e erec' @ E {{ Φ }}
+  ⊢ WP App e el @ E {{ Φ }}.
+Proof.
+  intros -> ??.
+  rewrite-(wp_lift_pure_det_head_step (App _ _) (subst f (Rec f xl erec) erec') None)
+          ?right_id //=.
+  intros; inv_head_step; eauto.
+Qed.
+
+Lemma wp_bin_op E op l1 l2 l' Φ :
+  bin_op_eval op l1 l2 = Some l' →
+  ▷ Φ (LitV l') ⊢ WP BinOp op (Lit l1) (Lit l2) @ E {{ Φ }}.
+Proof.
+  intros Heval. rewrite -(wp_lift_pure_det_head_step (BinOp op _ _) (Lit l') None)
+    ?right_id -?wp_value //; intros; inv_head_step; eauto.
+Qed.
+
+Lemma wp_case E i e el Φ :
+  0 ≤ i →
+  List.nth_error el (Z.to_nat i) = Some e →
+  ▷ WP e @ E {{ Φ }} ⊢ WP Case (Lit $ LitInt i) el @ E {{ Φ }}.
+Proof.
+  intros. rewrite -(wp_lift_pure_det_head_step (Case _ _) e None) ?right_id //.
+  intros; inv_head_step; auto.
+Qed.
+End lifting.
